HOL_To_IMP-/Refinements/HOL_To_IMP_Minus_Primitives.thy
@@ -472,9 +472,7 @@ compile_nat fun_pow_snd_nat_eq
 HOL_To_IMP_Minus_correct HTHN.fun_pow_snd_nat_nat
   supply Rel_nat_selector_Suc[Rel_nat]
   apply (tactic \<open>HM.correct_if_IMP_tailcall_correct_tac HT.get_IMP_def @{context} 1\<close>)
-  by (induction y arbitrary: ya s rule: nat.induct)
-  (tactic \<open>HT.start_run_finish_case_tac HT.get_IMP_def HT.get_imp_minus_correct
-    HB.get_HOL_eqs @{context} 1\<close>)+
+  by (induction y arbitrary: ya s rule: nat.induct) (cook mode = run_finish)
 
 compile_nat HTHN.nat_selector_eq_nat
 HOL_To_IMP_Minus_correct nat_selector by cook
